src/typechecker/FStar.TypeChecker.Tc.fst
@@ -865,24 +865,24 @@ let tc_decl' env0 se: list sigelt * list sigelt * Env.env =
     let se = ({ se with sigel = Sig_polymonadic_bind (m, n, p, t, ty, Some k) }) in
     [se], [], env0
 
-  | Sig_polymonadic_subcomp (m, n, t, _) ->  //desugaring does not set the last field, tc does
+  | Sig_polymonadic_subcomp (m, n, t, _, _) ->  //desugaring does not set the last field, tc does
     let t =
       if do_two_phases env then
         let t, ty =
           TcEff.tc_polymonadic_subcomp ({ env with phase1 = true; lax = true }) m n t
-          |> (fun (t, ty) -> { se with sigel = Sig_polymonadic_subcomp (m, n, t, ty) })
+          |> (fun (t, ty, _) -> { se with sigel = Sig_polymonadic_subcomp (m, n, t, ty, None) })
           |> N.elim_uvars env
           |> (fun se ->
              match se.sigel with
-             | Sig_polymonadic_subcomp (_, _, t, ty) -> t, ty
+             | Sig_polymonadic_subcomp (_, _, t, ty, _) -> t, ty
              | _ -> failwith "Impossible! tc for Sig_polymonadic_subcomp must be a Sig_polymonadic_subcomp") in
         if Env.debug env <| Options.Other "TwoPhases"
           then BU.print1 "Polymonadic subcomp after phase 1: %s\n"
-                 (Print.sigelt_to_string ({ se with sigel = Sig_polymonadic_subcomp (m, n, t, ty) }));
+                 (Print.sigelt_to_string ({ se with sigel = Sig_polymonadic_subcomp (m, n, t, ty, None) }));
         t
       else t in
-    let t, ty = TcEff.tc_polymonadic_subcomp env m n t in
-    let se = ({ se with sigel = Sig_polymonadic_subcomp (m, n, t, ty) }) in
+    let t, ty, k = TcEff.tc_polymonadic_subcomp env m n t in
+    let se = ({ se with sigel = Sig_polymonadic_subcomp (m, n, t, ty, Some k) }) in
     [se], [], env0)
 
 
@@ -958,7 +958,7 @@ let add_sigelt_to_env (env:Env.env) (se:sigelt) (from_cache:bool) : Env.env =
 
     | Sig_polymonadic_bind (m, n, p, _, ty, k) -> TcUtil.update_env_polymonadic_bind env m n p ty (k |> must)
 
-    | Sig_polymonadic_subcomp (m, n, _, ty) -> Env.add_polymonadic_subcomp env m n ty
+    | Sig_polymonadic_subcomp (m, n, _, ty, k) -> Env.add_polymonadic_subcomp env m n (ty, k |> must)
 
     | _ -> env
 
