src/typechecker/FStar.TypeChecker.TcEffect.fsti
@@ -35,4 +35,4 @@ val tc_effect_abbrev : Env.env -> (lident * S.univ_names * S.binders * S.comp) -
 
 val tc_polymonadic_bind : Env.env -> m:lident -> n:lident -> p:lident -> bind_t:S.tscheme -> S.tscheme & S.tscheme & S.indexed_effect_combinator_kind
 
-val tc_polymonadic_subcomp : Env.env -> m:lident -> n:lident -> subcomp_t:S.tscheme -> S.tscheme * S.tscheme
+val tc_polymonadic_subcomp : Env.env -> m:lident -> n:lident -> subcomp_t:S.tscheme -> S.tscheme & S.tscheme & S.indexed_effect_combinator_kind
